src/interop/py/Full/Random.py
@@ -16,8 +16,3 @@ class Random(DafnyVMCPart.Random):
     DafnyVMCPart.Random.Shuffle(self, a)
     return list(a)
   
-  def Shuffle32(self, xs):
-    a = ArrayFromList(xs)
-    DafnyVMCPart.Random.Shuffle32(self, a)
-    return list(a)
-  
