docs/dafny/ExamplesRandom.dfy
@@ -119,22 +119,12 @@ module Examples {
     print "Estimated probabilities for DiscreteGaussianSample(1.4): ", count0 as real / n as real, " (should be around 0.284959) and ", count1 as real / n as real, ", ", countneg1 as real / n as real, " (should both be around 0.220797)\n";
   
     // Fisher-Yates Shuffle Example
-    print "(Shuffle) Ten permutations of 012: ";
+    print "Ten permutations of 012: ";
     var arr: array<nat> := new nat[3](i => i); // [0, 1, 2]
     for i := 0 to 10 {
       var arrCopy := arr;
       r.Shuffle(arrCopy);
       print Helper.SeqToString(arrCopy[..], Helper.NatToString), ", ";
-    }
-    print "\n";
-
-    // Fisher-Yates Shuffle32 Example
-    print "(Shuffle 32) Ten permutations of 012: ";
-    var arr32: array<nat> := new nat[3](i => i); // [0, 1, 2]
-    for i := 0 to 10 {
-      var arrCopy32 := arr32;
-      r.Shuffle32(arrCopy32);
-      print Helper.SeqToString(arrCopy32[..], Helper.NatToString), ", ";
     }
     print "\n";
   }
