src/Util/FisherYates/Implementation.dfy
@@ -13,43 +13,7 @@ module FisherYates.Implementation {
 
   trait {:termination false} Trait extends Interface.Trait {
 
-    method Shuffle<T>(a: array<T>)
-      decreases *
-      modifies `s, a
-      ensures Model.Shuffle(old(a[..]))(old(s)) == Monad.Result(a[..], s)
-    {
-      ghost var prevI, prevASeq, prevS := 0, a[..], s; // ghost
-      if a.Length > 1 {
-        for i := 0 to a.Length - 1
-          invariant Equivalence.LoopInvariant(prevI, i, a, prevASeq, old(a[..]), old(s), prevS, s) // ghost
-        {
-          prevI, prevASeq, prevS := i, a[..], s; // ghost
-          var j := UniformIntervalSample(i, a.Length);
-          assert prevASeq == a[..]; // ghost
-          Swap(a, i, j);
-        }
-      } else {
-        Equivalence.ShuffleElseClause(a, old(a[..]), old(s), s); // ghost
-      }
-
-    }
-
-    method Swap<T>(a: array<T>, i: nat, j: nat)
-      modifies a
-      requires i <= j
-      requires 0 <= i < a.Length
-      requires 0 <= j < a.Length
-      ensures Model.Swap(old(a[..]), i, j) == a[..]
-      ensures old(s) == s
-    {
-      a[i], a[j] := a[j], a[i];
-    }
-
-  }
-
-  trait {:termination false} Trait32 extends Interface.Trait32 {
-
-    method {:vcs_split_on_every_assert} Shuffle32<T>(a: array<T>)
+    method {:vcs_split_on_every_assert} Shuffle<T>(a: array<T>)
       decreases *
       modifies `s, a
       requires a.Length < 0x8000_0000
@@ -59,12 +23,12 @@ module FisherYates.Implementation {
 
       if (a.Length as nat32) > (1 as nat32) {
         for i: nat32 := (0 as nat32) to (a.Length as nat32) - (1 as nat32)
-          invariant Equivalence.LoopInvariant32(prevI, i, a, prevASeq, old(a[..]), old(s), prevS, s) // ghost
+          invariant Equivalence.LoopInvariant(prevI, i, a, prevASeq, old(a[..]), old(s), prevS, s) // ghost
         {
           prevI, prevASeq, prevS := i, a[..], s; // ghost
           var j := UniformIntervalSample32(i, a.Length as nat32);
           assert prevASeq == a[..]; // ghost
-          Swap32(a, i, j);
+          Swap(a, i, j);
         }
       } else {
         Equivalence.ShuffleElseClause(a, old(a[..]), old(s), s); // ghost
@@ -72,7 +36,7 @@ module FisherYates.Implementation {
 
     }
 
-    method Swap32<T>(a: array<T>, i: nat32, j: nat32)
+    method Swap<T>(a: array<T>, i: nat32, j: nat32)
       modifies a
       requires i <= j
       requires 0 <= i as nat < a.Length
