tests/Tests.dfy
@@ -282,38 +282,6 @@ module Tests {
     modifies r
     modifies a
     requires n > 0
-  {
-    var a := new (T, nat)[a.Length](i reads a requires 0 <= i < a.Length => (a[i], i));
-    var numberOfPermutations: nat := NatArith.FactorialTraditional(a.Length);
-    var numberOfObservedPermutations: map<seq<(T, nat)>, nat> := map[];
-    
-    for i := 0 to n {
-      var aCopy := a;
-      r.Shuffle(aCopy);
-      var aCopyAsSeq := aCopy[..];
-      if aCopyAsSeq in numberOfObservedPermutations {
-        numberOfObservedPermutations := numberOfObservedPermutations[aCopyAsSeq := numberOfObservedPermutations[aCopyAsSeq] + 1];
-      } else {
-        numberOfObservedPermutations := numberOfObservedPermutations[aCopyAsSeq := 1];
-      }
-    }
-
-    var items := numberOfObservedPermutations.Items;
-
-    while items != {}
-      decreases |items| 
-     {
-      var item :| item in items;
-      items := items - {item};
-      TestBernoulliIsWithin3SigmaOfTrueMean(n, item.1 as real, 1.0 / numberOfPermutations as real, "p(" + Helper.SeqToString(item.0, printer) + ")");
-    }
-  }
-
-  method TestFisherYates32<T(==, !new)>(n: nat, a: array<T>, r: DafnyVMC.Random, printer: ((T, nat)) -> string) 
-    decreases *
-    modifies r
-    modifies a
-    requires n > 0
     requires a.Length < 0x8000_0000
   {
     var a := new (T, nat)[a.Length](i reads a requires 0 <= i < a.Length => (a[i], i));
@@ -322,7 +290,7 @@ module Tests {
     
     for i := 0 to n {
       var aCopy := a;
-      r.Shuffle32(aCopy);
+      r.Shuffle(aCopy);
       var aCopyAsSeq := aCopy[..];
       if aCopyAsSeq in numberOfObservedPermutations {
         numberOfObservedPermutations := numberOfObservedPermutations[aCopyAsSeq := numberOfObservedPermutations[aCopyAsSeq] + 1];
