build/java/run_shuffling.sh
@@ -1,4 +1,3 @@
 #1/bin/bash
 
 java -classpath build/java/DafnyVMC.jar docs/java/TestShuffling.java
-java -classpath build/java/DafnyVMC.jar docs/java/TestShuffling32.java
